Foundation/IntProp/Kripke/LEM.lean
@@ -1,150 +1,202 @@
 import Foundation.IntProp.Kripke.Semantics
 
-/-!
-  # Counterexample to the Law of Excluded Middle in Intuitionistic Logic
-
-  ## Theorems
-  - `noLEM`: LEM is not always valid in intuitionistic logic.
--/
+-- TODO: prove `Formula.Kripke.ValidOnFrame.subst`
 
 namespace LO.IntProp
 
 open System
 open Formula Formula.Kripke
 
-
-variable {α : Type u}
-
-abbrev NoLEMFrame : Kripke.Frame where
-  World := PUnit ⊕ PUnit
-  Rel x y :=
-    match x, y with
-    | .inl _, .inl _ => True
-    | .inr _, .inr _ => True
-    | .inl _, .inr _ => True
-    | _, _ => False
-
-namespace NoLEMFrame
-
-lemma is_transitive : Transitive NoLEMFrame.Rel := by simp [Transitive];
-
-lemma is_reflexive : Reflexive NoLEMFrame.Rel := by simp [Reflexive];
-
-lemma is_confluent : Confluent NoLEMFrame.Rel := by simp [Confluent];
-
-lemma is_connected : Connected NoLEMFrame.Rel := by simp [Connected];
-
-end NoLEMFrame
-
-
-lemma Kripke.noLEM_on_frameclass [Inhabited α] : ∃ (φ : Formula α), ¬((Kripke.FrameClassOfHilbert.{u, 0} (Hilbert.Int α)) ⊧ φ ⋎ ∼φ) := by
-  use (atom default);
-  simp [Semantics.Realize];
-  use NoLEMFrame;
-  constructor;
-  . apply Int_Characteraizable.characterize;
-    exact ⟨NoLEMFrame.is_reflexive, NoLEMFrame.is_transitive⟩;
-  . simp [ValidOnFrame];
-    use (λ w _ => match w with | .inr _ => True | .inl _ => False);
+-- TODO: 成り立つのか？
+lemma Formula.Kripke.ValidOnFrame.subst {F : Kripke.Frame} {φ : Formula ℕ} (h : F ⊧ φ) (s : ℕ → Formula ℕ) : F ⊧ φ.subst s := by sorry;
+  /-
+  induction φ using Formula.rec' with
+  | hatom =>
+    intro V x;
+    refine h (V := ⟨λ x a => Satisfies ⟨F, V⟩ x (s a), ?_⟩) x;
+    intro x y Rxy a;
+    exact formula_hereditary Rxy;
+  | hverum => simp;
+  | hfalsum => simp at h;
+  | hand _ _ hφ hψ =>
+    intro V x;
+    apply Satisfies.and_def.mp;
     constructor;
-    . simp;
-    . simp [ValidOnModel, Satisfies];
+    . apply hφ;
+      intro V x;
+      exact h x |>.1;
+    . apply hψ;
+      intro V x;
+      exact h x |>.2;
+  | himp φ ψ hφ hψ =>
+    apply Satisfies.imp_def.mp;
+    intro y Rxy hy;
+    apply hψ;
+    intro V' z;
+    have := @h V x;
+    have := @Satisfies.imp_def ⟨F, V⟩ x φ ψ |>.mp this Rxy;
+    apply h;
+    . sorry;
+    . sorry;
+    sorry;
+  | hor φ ψ hφ hψ =>
+    intro V x;
+    rcases Satisfies.or_def.mp $ h x with (hl | hr);
+    . left;
+      apply hφ;
+      intro V' y;
+      sorry;
+    . sorry;
+  | hneg φ hφ =>
+    intro V x;
+    apply Satisfies.neg_def.mpr;
+    intro y Rxy hyφ;
+    have := @h V y;
+    apply hφ;
+  -/
 
+namespace Hilbert
 
-/--
-  Law of Excluded Middle is not always provable in intuitionistic logic.
--/
-theorem Hilbert.Int.noLEM [Inhabited α] : ∃ (φ : Formula α), (Hilbert.Int α) ⊬ φ ⋎ ∼φ := by
-  obtain ⟨φ, hp⟩ := Kripke.noLEM_on_frameclass (α := α);
-  use φ;
-  by_contra hC;
-  have := @Kripke.sound _ _ _ hC;
+open Kripke
+
+variable {a b : ℕ}
+
+theorem Int.no_WeakLEM : ∃ a, (Hilbert.Int ℕ) ⊬ Axioms.WeakLEM (atom a) := by
+  by_contra hC; simp at hC;
+  let F : Kripke.Frame := {
+    World := Fin 3
+    Rel := λ x y =>
+      match x, y with
+      | 0, _ => True
+      | x, y => x = y
+    rel_po := {
+      refl := by aesop;
+      antisymm := by aesop;
+      trans := by aesop;
+    }
+  }
+  have : Confluent F := by
+    apply @Kripke.ConfluentFrameClass.defined_by_WLEM F |>.mpr;
+    simp [Semantics.RealizeSet.setOf_iff, ValidOnFrame.models_iff];
+    intro φ;
+    suffices ValidOnFrame F (Axioms.WeakLEM (atom 0))
+      from @Formula.Kripke.ValidOnFrame.subst F (Axioms.WeakLEM (atom 0)) this (λ a => match a with | 0 => φ | _ => atom a);
+    apply (Hilbert.Int.Kripke.sound.sound $ hC 0) F;
+    tauto;
+  have : ¬Confluent F := by
+    simp only [Confluent]; push_neg;
+    use 0, 1, 2;
+    simp;
   contradiction;
 
-/--
-  Intuitionistic logic is proper weaker than classical logic.
--/
-theorem Hilbert.Int_strictly_weaker_than_Cl [DecidableEq α] [Inhabited α] : (Hilbert.Int α) <ₛ (Hilbert.Cl α) := by
+theorem Int_strictly_weaker_than_LC : (Hilbert.Int ℕ) <ₛ (Hilbert.KC ℕ) := by
   constructor;
-  . exact Hilbert.Int_weaker_than_Cl;
-  . apply weakerThan_iff.not.mpr;
+  . exact Hilbert.Int_weaker_than_KC;
+  . obtain ⟨a, h⟩ := Int.no_WeakLEM;
+    apply weakerThan_iff.not.mpr;
     push_neg;
-    obtain ⟨φ, hp⟩ := Hilbert.Int.noLEM (α := α);
-    use (φ ⋎ ∼φ);
+    use ∼(atom a) ⋎ ∼∼(atom a);
     constructor;
-    . exact lem!;
-    . assumption;
+    . exact wlem!;
+    . exact h;
 
-
-section
-
-lemma Kripke.noLEM_on_frameclass_KC [DecidableEq α] [Inhabited α]  : ∃ (φ : Formula α), ¬((Kripke.FrameClassOfHilbert.{u, 0} (Hilbert.KC α)) ⊧ φ ⋎ ∼φ) := by
-  use (atom default);
-  simp [Semantics.Realize];
-  use NoLEMFrame;
-  constructor;
-  . apply Kripke.KC_Characteraizable.characterize;
-    exact ⟨NoLEMFrame.is_reflexive, NoLEMFrame.is_transitive, NoLEMFrame.is_confluent⟩;
-  . simp [ValidOnFrame];
-    use (λ w _ => match w with | .inr _ => True | .inl _ => False);
-    constructor;
-    . simp;
-    . simp [ValidOnModel, Satisfies];
-
-lemma Hilbert.KC.noLEM [DecidableEq α] [Inhabited α] : ∃ (φ : Formula α), (Hilbert.KC α) ⊬ φ ⋎ ∼φ := by
-  obtain ⟨φ, hp⟩ := Kripke.noLEM_on_frameclass_KC (α := α);
-  use φ;
-  by_contra hC;
-  have := @Kripke.sound _ _ _ hC;
+theorem KC.no_Dummett : ∃ a b, (Hilbert.KC ℕ) ⊬ Axioms.Dummett (atom a) (atom b) := by
+  by_contra hC; simp at hC;
+  let F : Kripke.Frame := {
+    World := Fin 4
+    Rel := λ x y =>
+      match x, y with
+      | 1, 2 => False
+      | x, y => x ≤ y
+    rel_po := {
+      refl := by simp only [le_refl, implies_true];
+      trans := by
+        intro x y z Rxy Ryx;
+        split at Rxy;
+        . contradiction;
+        . split at Ryx;
+          . contradiction;
+          . split;
+            . simp_all; omega;
+            . omega;
+      antisymm := by
+        intro x y Rxy Ryx;
+        split at Rxy;
+        . contradiction;
+        . split at Ryx;
+          . contradiction;
+          . exact LE.le.antisymm Rxy Ryx;
+    }
+  };
+  have : Connected F := by
+    apply @Kripke.ConnectedFrameClass.defined_by_Dummett F |>.mpr;
+    simp [Semantics.RealizeSet.setOf_iff, ValidOnFrame.models_iff];
+    rintro _ φ ψ rfl;
+    suffices ValidOnFrame F (Axioms.Dummett (atom 0) (atom 1))
+      from @Formula.Kripke.ValidOnFrame.subst F (Axioms.Dummett (atom 0) (atom 1)) this (λ a => match a with | 0 => φ | 1 => ψ | _ => atom a);
+    apply (Hilbert.KC.Kripke.sound.sound $ hC 0 1) F;
+    simp [Confluent];
+    intro x y z Rxy Ryz;
+    use 3;
+    split at Rxy;
+    . contradiction;
+    . split at Ryz;
+      . contradiction;
+      . constructor;
+        . simp_all; omega;
+        . simp_all; omega;
+  have : ¬Connected F := by
+    simp only [Connected]; push_neg;
+    use 0, 1, 2;
+    simp;
   contradiction;
 
-theorem Hilbert.KC_strictly_weaker_than_Cl [DecidableEq α] [Inhabited α] : (Hilbert.KC α) <ₛ (Hilbert.Cl α) := by
+theorem KC_strictly_weaker_than_LC : (Hilbert.KC ℕ) <ₛ (Hilbert.LC ℕ) := by
   constructor;
-  . exact Hilbert.KC_weaker_than_Cl;
-  . apply weakerThan_iff.not.mpr;
+  . exact Hilbert.KC_weaker_than_LC;
+  . obtain ⟨a, b, h⟩ := KC.no_Dummett;
+    apply weakerThan_iff.not.mpr;
     push_neg;
-    obtain ⟨φ, hp⟩ := Hilbert.KC.noLEM (α := α);
-    use (φ ⋎ ∼φ);
+    use Axioms.Dummett (atom a) (atom b);
     constructor;
-    . exact lem!;
-    . assumption;
+    . exact dummett!;
+    . exact h;
 
-end
-
-
-section
-
-lemma Kripke.noLEM_on_frameclass_LC [Inhabited α] : ∃ (φ : Formula α), ¬((Kripke.FrameClassOfHilbert.{u, 0} (Hilbert.LC α)) ⊧ φ ⋎ ∼φ) := by
-  use (atom default);
-  simp [Semantics.Realize];
-  use NoLEMFrame;
-  constructor;
-  . apply LC_Characteraizable.characterize;
-    exact ⟨NoLEMFrame.is_reflexive, NoLEMFrame.is_transitive, NoLEMFrame.is_connected⟩;
-  . simp [ValidOnFrame];
-    use (λ w _ => match w with | .inr _ => True | .inl _ => False);
-    constructor;
-    . simp;
-    . simp [ValidOnModel, Satisfies];
-
-lemma Hilbert.LC.noLEM [Inhabited α] : ∃ (φ : Formula α), (Hilbert.LC α) ⊬ φ ⋎ ∼φ := by
-  obtain ⟨φ, hp⟩ := Kripke.noLEM_on_frameclass_LC (α := α);
-  use φ;
-  by_contra hC;
-  have := @Kripke.sound _ _ _ hC;
+theorem LC.no_LEM : ∃ a, (Hilbert.LC ℕ) ⊬ Axioms.LEM (atom a) := by
+  by_contra hC; simp at hC;
+  let F : Kripke.Frame := {
+    World := Fin 2
+    Rel := λ x y => x ≤ y
+  };
+  have : Euclidean F := by
+    apply @Kripke.EuclideanFrameClass.defined_by_LEM F |>.mpr;
+    simp [Semantics.RealizeSet.setOf_iff, ValidOnFrame.models_iff];
+    intro φ;
+    suffices ValidOnFrame F (Axioms.LEM (atom 0))
+      from @Formula.Kripke.ValidOnFrame.subst F (Axioms.LEM (atom 0)) this (λ a => match a with | 0 => φ | _ => atom a);
+    apply (Hilbert.LC.Kripke.sound.sound $ hC 0) F;
+    simp [Connected];
+    omega;
+  have : ¬Euclidean F := by
+    simp only [Euclidean]; push_neg;
+    use 0, 0, 1;
+    simp;
   contradiction;
 
-theorem Hilbert.LC_strictly_weaker_than_Cl [DecidableEq α] [Inhabited α] : (Hilbert.LC α) <ₛ (Hilbert.Cl α) := by
+theorem LC_strictly_weaker_than_Cl : (Hilbert.LC ℕ) <ₛ (Hilbert.Cl ℕ) := by
   constructor;
   . exact Hilbert.LC_weaker_than_Cl;
-  . apply weakerThan_iff.not.mpr;
+  . obtain ⟨a, h⟩ := LC.no_LEM;
+    apply weakerThan_iff.not.mpr;
     push_neg;
-    obtain ⟨φ, hp⟩ := Hilbert.LC.noLEM (α := α);
-    use (φ ⋎ ∼φ);
+    use Axioms.LEM (atom a);
     constructor;
     . exact lem!;
-    . assumption;
+    . exact h;
 
-end
+theorem Int_strictly_weaker_than_Cl : (Hilbert.Int ℕ) <ₛ (Hilbert.Cl ℕ) :=
+  strictlyWeakerThan.trans Int_strictly_weaker_than_LC $ strictlyWeakerThan.trans KC_strictly_weaker_than_LC LC_strictly_weaker_than_Cl
+
+end Hilbert
 
 end LO.IntProp
